@prefix : <http://material-digital.de/pmdao/hto/> .
@prefix owl: <http://www.w3.org/2002/07/owl#> .
@prefix rdf: <http://www.w3.org/1999/02/22-rdf-syntax-ns#> .
@prefix sdo: <http://schema.org/> .
@prefix xml: <http://www.w3.org/XML/1998/namespace> .
@prefix xsd: <http://www.w3.org/2001/XMLSchema#> .
@prefix rdfs: <http://www.w3.org/2000/01/rdf-schema#> .
@prefix pmdco: <http://material-digital.de/pmdco/> .
@base <http://material-digital.de/pmdao/hto/> .

<http://material-digital.de/pmdao/hto/> rdf:type owl:Ontology ;
                                         owl:versionIRI <http://material-digital.de/pmdao/hto/1.0> ;
                                         owl:imports pmdco: ;
                                         <http://purl.org/dc/elements/1.1/creator> <https://orcid.org/0000-0002-9014-2920> ,
                                                                                   "Jannis Grundmann" ,
                                                                                   "https://orcid.org/0000-0003-4461-6539" ;
                                         <http://purl.org/dc/elements/1.1/title> "Heat Treatment Ontology (HTO)"@en ;
                                         owl:versionInfo "1.0"^^xsd:string ;
                                         <http://www.w3.org/2004/02/skos/core#definition> "This is a pre version of the PMD application ontology (PMDao) of generic heat treatments (Heat Treatment Ontology - HTO)."@en ;
                                         <http://www.w3.org/ns/prov#editorialNote> "The heat treatment ontology (HTO) is developed in the context of the joint project of platform material digital (PMD). The HTO is connected to the PMD core ontology (PMDco)."@en .

#################################################################
#    Annotation properties
#################################################################

###  http://purl.org/dc/elements/1.1/creator
<http://purl.org/dc/elements/1.1/creator> rdf:type owl:AnnotationProperty .


###  http://purl.org/dc/elements/1.1/title
<http://purl.org/dc/elements/1.1/title> rdf:type owl:AnnotationProperty .


###  http://www.w3.org/2004/02/skos/core#definition
<http://www.w3.org/2004/02/skos/core#definition> rdf:type owl:AnnotationProperty .


###  http://www.w3.org/2004/02/skos/core#example
<http://www.w3.org/2004/02/skos/core#example> rdf:type owl:AnnotationProperty .


###  http://www.w3.org/ns/prov#editorialNote
<http://www.w3.org/ns/prov#editorialNote> rdf:type owl:AnnotationProperty .


#################################################################
#    Classes
#################################################################

###  http://material-digital.de/pmdao/hto/Carburizing
:Carburizing rdf:type owl:Class ;
             rdfs:subClassOf :Holding ;
             rdfs:comment "Notiz: potentiell ableitbar mit bestimmten Fluss-Schwellenwerten"@de ,
                          "Process step during which carbon is transferred from the atmosphere to the component surface."@en ,
                          "Prozessschritt, während dessen Kohlenstoff aus der Atmosphäre an der Bauteiloberfläche übertragen wird"@de ;
             rdfs:label "Aufkohlen"@de ,
                        "Carburizing"@en .


###  http://material-digital.de/pmdao/hto/CoolingProcess
:CoolingProcess rdf:type owl:Class ;
                rdfs:subClassOf pmdco:HeatTreatmentProcess ;
                rdfs:comment "A process in which the temperature is lowered from a higher to a lower level."@en ,
                             "Ein Prozess, bei dem die Temperatur von einem höherem auf ein niedrigeres Niveau abgesenkt wird."@de ;
                rdfs:label "Abkühlprozess"@de ,
                           "Cooling Process"@en .


###  http://material-digital.de/pmdao/hto/DurationTillTargetTemperature
:DurationTillTargetTemperature rdf:type owl:Class ;
                               rdfs:subClassOf pmdco:Duration ;
                               rdfs:comment "Erwärmdauer = Heizzeit + Durchwärmdauer"@de ,
                                            "Maß für die tatsächliche Dauer eines Erwärmvorgangs."@de ,
                                            "Measurement representing the actual duration of a heating procedure."@en ;
                               rdfs:label "Duration Till Target Temperature"@en ,
                                          "Erwärmdauer"@de .


###  http://material-digital.de/pmdao/hto/Flow
:Flow rdf:type owl:Class ;
      rdfs:subClassOf pmdco:ValueObject ;
      rdfs:comment "Value Object representing the intended induced flow rate of a medium."@en ;
      rdfs:label "Flow"@en ;
      <http://www.w3.org/2004/02/skos/core#example> """vo1 a ValueObject ,
          Flow ,
          Setpoint , 
          Metadata .

vo1 relatesTo CHEBI:Argon .

vo1 hasValue 29.2 ;
       hasUnit qudt:LitrePerHour ."""@en .


###  http://material-digital.de/pmdao/hto/HardeningProcess
:HardeningProcess rdf:type owl:Class ;
                  rdfs:subClassOf :HeatTreatmentType ;
                  rdfs:comment "Heat treatment process with the aim of achieving an increase in strength."@en ,
                               "Wärmebehandlungprozess mit dem Ziel eine Festigkeitssteigerung zu erreichen."@de ;
                  rdfs:label "Hardening Process"@en ,
                             "Härten"@de .


###  http://material-digital.de/pmdao/hto/HeatTreatmentChamber
:HeatTreatmentChamber rdf:type owl:Class ;
                      rdfs:subClassOf pmdco:ProcessingNode ;
                      rdfs:comment "Functional furnace chamber."@en ,
                                   "Funktionale Ofenkammer."@de ,
                                   "Notiz: Sollte mit Unit-Volume (m^3) verbunden sein"@de ;
                      rdfs:label "Heat Treatment Chamber"@en ,
                                 "Wärmebehandlungsofenkammer"@de .


###  http://material-digital.de/pmdao/hto/HeatTreatmentFurnace
:HeatTreatmentFurnace rdf:type owl:Class ;
                      rdfs:subClassOf pmdco:ProcessingNode ;
                      rdfs:comment "A furnace intended to change the physical and chemical properties of objects (e.g., test pieces or blanks) achieved through heat treatment techniques such as annealing, case hardening, precipitation, strengthening, tempering, normalizing, or quenching."@en ;
                      rdfs:label "Ein Ofen, der dazu bestimmt ist, die physikalischen und chemischen Eigenschaften von Objekten (z. B. Prüfstücke oder Rohlinge) durch Wärmebehandlungsverfahren wie Glühen, Einsatzhärten, Nitrieren, Borieren, Ausscheidungsbildung, Verfestigen, Anlassen, Normalisieren oder Abschrecken zu verändern."@de ,
                                 "Heat Treatment Furnace"@en ,
                                 "Wärmebehandlungsofen"@de .


###  http://material-digital.de/pmdao/hto/HeatTreatmentOverheat
:HeatTreatmentOverheat rdf:type owl:Class ;
                       rdfs:subClassOf pmdco:Temperature ;
                       rdfs:comment "Maximal zulässige Abweichung einer Ist-Temperatur, die die Aufheiz-Soll-Temperatur überschreitet. Die Überhitzung kann absichtlich höher als die vorgesehene Aufheiz-Soll-Temperatur eingestellt werden, um die Temperatur eines Objekts implizit zu steuern (in der Annahme, dass ein Objekt kühler ist als die gemessene Ofentemperatur)."@de ,
                                    "Maximum allowed deviation of a actual temperature that exceeds the heatup-target temperature. Overheat may be set higher than the intended heatup-target temperature deliberatly in order to implictly control an object's temperature (based on the assumption that an object is cooler than the measured furnace temperature)."@en ;
                       rdfs:label "Heat Treatment Overheat"@en ,
                                  "Übertemperatur"@de .


###  http://material-digital.de/pmdao/hto/HeatTreatmentType
:HeatTreatmentType rdf:type owl:Class ;
                   rdfs:subClassOf pmdco:ConditioningProcess ;
                   rdfs:label "Heat Treatment Type"@en .


###  http://material-digital.de/pmdao/hto/HeatingChamber
:HeatingChamber rdf:type owl:Class ;
                rdfs:subClassOf :HeatTreatmentChamber ;
                rdfs:comment "Distinguishable chamber of a heat treatment furnace with a heater."@en ;
                rdfs:label "Heating Chamber"@en ,
                           "Heizkammer"@de ,
                           "Ofenkammer mit einer Heizung."@de .


###  http://material-digital.de/pmdao/hto/HeatingProcess
:HeatingProcess rdf:type owl:Class ;
                rdfs:subClassOf pmdco:HeatTreatmentProcess ;
                rdfs:comment "A process in which the temperature is increased from a lower to a higher level."@en ,
                             "Ein Prozess, bei dem die Temperatur von einem niedrigem auf ein höheres Niveau gesteigert wird."@de ;
                rdfs:label "Erwärmprozess"@de ,
                           "Heating Process"@en .


###  http://material-digital.de/pmdao/hto/HeatingTime
:HeatingTime rdf:type owl:Class ;
             rdfs:subClassOf pmdco:Duration ;
             rdfs:comment "Dauer bis zum Erreichen der Zieltemperatur im Ofen."@de ,
                          "Duration until the target temperature is reached in the furnace."@en ;
             rdfs:label "Erwärmdauer"@de ,
                        "Heating Time"@en .


###  http://material-digital.de/pmdao/hto/Holding
:Holding rdf:type owl:Class ;
         rdfs:subClassOf pmdco:HeatTreatmentProcess ;
         rdfs:comment "Process step without temperature change in the furnace."@en ,
                      "Prozessschritt ohne Temperaturänderung im Ofen."@de ;
         rdfs:label "Halten"@de ,
                    "Holding"@en .


###  http://material-digital.de/pmdao/hto/OilQuenchingDuration
:OilQuenchingDuration rdf:type owl:Class ;
                      rdfs:subClassOf pmdco:Duration ;
                      rdfs:comment "Dwell time of the components in the quenching medium."@en ,
                                   "Verweildauer der Bauteile im Abschreckmedium."@de ;
                      rdfs:label "Abschreckdauer"@de ,
                                 "Oil Quenching Duration"@en .


###  http://material-digital.de/pmdao/hto/OilTemperature
:OilTemperature rdf:type owl:Class ;
                rdfs:subClassOf pmdco:EnvironmentalTemperature ;
                rdfs:comment "Am Anfang der Abschreckung vorliegenden Temperatur des Abschreckmediums."@de ,
                             "The temperature of the quenching medium at the start of quenching."@en ;
                rdfs:label "Abschreckmediumtemperatur"@de ,
                           "Media Temperature"@en ;
                <http://www.w3.org/2004/02/skos/core#example> """oil a Medium ;
   hasCharacterstic vo1 ;
   relatesTo CHEBI:XXXX .

vo1 a ValueObject ,
          Temperature ,
          Setpoint , 
          Metadata ;
      hasValue 60.0 ;
      hasUnit qudt:DegreeCelsius ."""@en .


###  http://material-digital.de/pmdao/hto/PartialPressure
:PartialPressure rdf:type owl:Class ;
                 rdfs:subClassOf :Pressure ;
                 rdfs:comment "Describing the intended pressure inside a chamber targeted in a factor relative to one bar (using a vakuum cooling or an atmosphere flow)."@en ,
                              "The complement to vacuum-heating as it allows for active vacuum pump during atmosphere flow. Should be set to zero, if vacuum-heating is true."@en ;
                 rdfs:label "Partial Pressure"@en .


###  http://material-digital.de/pmdao/hto/Pressure
:Pressure rdf:type owl:Class ;
          rdfs:subClassOf pmdco:ValueObject ;
          rdfs:comment """Pressure (symbol: p or P) is the force applied perpendicular to the surface of an object per unit area over which that force is distributed.
https://en.wikipedia.org/wiki/Pressure"""@en ;
          rdfs:label "Pressure"@en .


###  http://material-digital.de/pmdao/hto/QuenchingChamber
:QuenchingChamber rdf:type owl:Class ;
                  rdfs:subClassOf :HeatTreatmentChamber ;
                  rdfs:comment "Chamber of a heat treatment furnace that is designed to quench objects."@en ;
                  rdfs:label "Abschreckkammer"@de ,
                             "Kammer eines Wärmebehandlungsofens, die zum Abschrecken von Gegenständen bestimmt ist."@de ,
                             "Quenching Chamber"@en .


###  http://material-digital.de/pmdao/hto/QuenchingLeadtime
:QuenchingLeadtime rdf:type owl:Class ;
                   rdfs:subClassOf pmdco:Duration ;
                   rdfs:comment "Dauer zwischen Verlassen der Heizkammer und Beginn der effektiven Abschreckung. Gilt für Zweikammeröfen."@de ,
                                "Duration between leaving the heating chamber and the start of effective quenching. Applies to two-chamber furnaces."@en ;
                   rdfs:label "Abschreckvorlaufzeit"@de ,
                              "Quenching Leadtime"@en .


###  http://material-digital.de/pmdao/hto/QuenchingProcess
:QuenchingProcess rdf:type owl:Class ;
                  rdfs:subClassOf :CoolingProcess ;
                  rdfs:comment "Process with significantly increased cooling rate, aimed at preventing certain structural transformations."@en ,
                               "Prozess mit stark erhöhter Abkühlgeschwindigkeit, mit dem Ziel der Verhinderung bestimmter Gefügeumwandlungen."@de ;
                  rdfs:label "Abschreckprozess"@de ,
                             "Quenching Process"@en .


###  http://material-digital.de/pmdao/hto/SoakingLeadTime
:SoakingLeadTime rdf:type owl:Class ;
                 rdfs:subClassOf pmdco:Duration ;
                 rdfs:comment "Dauer bis zum Erreichen der homogenen Temperatur im Bauteil."@de ,
                              "Duration until the homogeneous temperature is reached in the component."@en ;
                 rdfs:label "Durchwärmzeit"@de ,
                            "Soaking Time"@en .


###  http://material-digital.de/pmdao/hto/SoakingProcess
:SoakingProcess rdf:type owl:Class ;
                rdfs:subClassOf :Holding ;
                rdfs:comment "Process step during which temperature homogenization is achieved in the component."@en ,
                             "Prozesschritt, während dessen die Temperaturhomogenisierung im Bauteil erreicht wird."@de ;
                rdfs:label "Durchwärmen"@de ,
                           "Soaking Process"@en .


###  http://material-digital.de/pmdao/hto/Status
:Status rdf:type owl:Class ;
        rdfs:subClassOf pmdco:NodeInfo ;
        rdfs:label "Status"@en .


###  http://material-digital.de/pmdao/hto/TargetTemperature
:TargetTemperature rdf:type owl:Class ;
                   rdfs:subClassOf pmdco:Temperature ;
                   rdfs:comment "Darstellung der beabsichtigten Zieltemperatur in Celsius am Ende eines Aufheizvorgangs."@de ,
                                "Representing the intended target temperature in celsius at the end of a heating process."@en ;
                   rdfs:label "Target Temperature"@en ,
                              "Zieltemperatur"@de .


###  http://material-digital.de/pmdao/hto/TemperatureChangeRate
:TemperatureChangeRate rdf:type owl:Class ;
                       rdfs:subClassOf pmdco:Temperature ;
                       rdfs:comment "Defined temperature change rate in temperature change per time unit."@en ,
                                    "Definierte Temperaturänderungsrate in Temperaturänderung pro Zeiteinheit."@de ,
                                    "[FIXME] Are two units appendable?"@en ;
                       rdfs:label "Temperature Change Rate"@en ,
                                  "Temperaturänderungsrate"@de .


###  http://material-digital.de/pmdao/hto/TemperingProcess
:TemperingProcess rdf:type owl:Class ;
                  rdfs:subClassOf :HeatTreatmentType ;
                  rdfs:comment "A heat treatment process to transform the hardening structure into the direction or equilibrium structure."@en ,
                               "Ein Wärmebehandlungsprozess, um das Härtungsgefüge in die Richtung oder in ein Gleichgewichtsgefüge umzuwandeln."@de ;
                  rdfs:label "Anlassen"@de ,
                             "Tempering Process"@en .


###  http://material-digital.de/pmdao/hto/TypeDescription
:TypeDescription rdf:type owl:Class ;
                 rdfs:subClassOf pmdco:NodeInfo ;
                 rdfs:comment "Description for Process Node's utility, e.g. \"Rear Vacuum Furnace Oil Quenching\""@en ;
                 rdfs:label "Typbeschreibung"@de ,
                            "Type Description"@en .


###  http://material-digital.de/pmdao/hto/VacuumHeatingPressure
:VacuumHeatingPressure rdf:type owl:Class ;
                       rdfs:subClassOf :Pressure ;
                       rdfs:comment "Pressure of the vaccum heating pump."@en ;
                       rdfs:label "Vacuum Heating Pressure"@en .


###  http://material-digital.de/pmdao/hto/hasConductedQuenchingAction
:hasConductedQuenchingAction rdf:type owl:Class ;
                             rdfs:subClassOf :Status ;
                             rdfs:comment "Boolean parameter indicating existence of \"Ölabschrecken_QK\" in primary data."@en ;
                             rdfs:label "has Conducted Quenching Action"@en .


###  http://material-digital.de/pmdao/hto/hasOilFlow
:hasOilFlow rdf:type owl:Class ;
            rdfs:subClassOf :Status ;
            rdfs:comment "Boolean parameter to control the oil circulation/agitation to increase the quenching rate."@en ;
            rdfs:label "has Oil Flow"@en .


###  http://material-digital.de/pmdao/hto/isFanFast
:isFanFast rdf:type owl:Class ;
           rdfs:subClassOf :Status ;
           rdfs:comment "Boolean parameter representing a fast fan speed setting in contrast to the default speed setting."@en ;
           rdfs:label "is Fan Fast"@en .


###  http://material-digital.de/pmdao/hto/isGasCooling
:isGasCooling rdf:type owl:Class ;
              rdfs:subClassOf :Status ;
              rdfs:comment "parameter, bool, modus of cooling a batch in the heating chamber, gasflow is possible."@en ;
              rdfs:label "is Gas Cooling"@en .


###  http://material-digital.de/pmdao/hto/isGasIngressBack
:isGasIngressBack rdf:type owl:Class ;
                  rdfs:subClassOf :Status ;
                  rdfs:comment "Boolean parameter that opens a magnetic-controlled valve to induce gas ingress from back (if set to true) into the heating chamber"@en ;
                  rdfs:label "is Gas Ingress Back"@en .


###  http://material-digital.de/pmdao/hto/isGasIngressFront
:isGasIngressFront rdf:type owl:Class ;
                   rdfs:subClassOf :Status ;
                   rdfs:comment "Boolean parameter that opens a magnetic-controlled valve to induce frontsited gas ingress (if set to true) into the heating chamber."@en ;
                   rdfs:label "is Gas Ingress Front"@en .


###  http://material-digital.de/pmdao/hto/isGasIngressIntermediate
:isGasIngressIntermediate rdf:type owl:Class ;
                          rdfs:subClassOf :Status ;
                          rdfs:comment "Boolean parameter that opens a magnetic-controlled valve to induce gas ingress from side (if set to true) into the heating chamber."@en ;
                          rdfs:label "is Gas Ingress Intermediate"@en .


###  http://material-digital.de/pmdao/hto/isOilFlowFast
:isOilFlowFast rdf:type owl:Class ;
               rdfs:subClassOf :Status ;
               rdfs:comment "Boolean parameter to control the oil circulation speed (slow/fast)."@en ;
               rdfs:label "is Oil Flow Fast"@en .


###  http://material-digital.de/pmdao/hto/isOilFlowUp
:isOilFlowUp rdf:type owl:Class ;
             rdfs:subClassOf :Status ;
             rdfs:comment "Boolean parameter"@en ;
             rdfs:label "is Oil Flow Up"@en .


###  http://material-digital.de/pmdao/hto/isQuenchingUpDown
:isQuenchingUpDown rdf:type owl:Class ;
                   rdfs:subClassOf :Status ;
                   rdfs:comment "Boolean parameter representing a specific quenching mode, immersing an object into and lifting it from the cooling fluid again."@en ;
                   rdfs:label "is Quenching Up Down"@en .


###  http://material-digital.de/pmdao/hto/isVacuumCooling
:isVacuumCooling rdf:type owl:Class ;
                 rdfs:subClassOf :Status ;
                 rdfs:comment "Parameter that sets the activity of the vacuum pump. If true, no atmosphere flow is possible (even if set). Effectively, the same mechanics as vacuum-heating (this is for humans)."@en ;
                 rdfs:label "is Vacuum Cooling"@en .


###  http://material-digital.de/pmdco/ConditioningProcess
pmdco:ConditioningProcess rdf:type owl:Class .


###  http://material-digital.de/pmdco/Duration
pmdco:Duration rdf:type owl:Class .


###  http://material-digital.de/pmdco/EnvironmentalTemperature
pmdco:EnvironmentalTemperature rdf:type owl:Class .


###  http://material-digital.de/pmdco/HeatTreatmentProcess
pmdco:HeatTreatmentProcess rdf:type owl:Class .


###  http://material-digital.de/pmdco/NodeInfo
pmdco:NodeInfo rdf:type owl:Class .


###  http://material-digital.de/pmdco/ProcessingNode
pmdco:ProcessingNode rdf:type owl:Class .


###  http://material-digital.de/pmdco/Temperature
pmdco:Temperature rdf:type owl:Class ;
                  rdfs:comment "Representing the intended temperature in celsius to hold."@en .


###  http://material-digital.de/pmdco/ValueObject
pmdco:ValueObject rdf:type owl:Class .


###  Generated by the OWL API (version 4.5.9.2019-02-01T07:24:44Z) https://github.com/owlcs/owlapi
